examples/delayed_echo/LinkedList01proof.v
@@ -1,0 +1,517 @@
+Require Import LinkedList0 LinkedList1 SimModSem HoareDef.
+Require Import Mem1.
+Require Import Coqlib.
+Require Import Universe.
+Require Import Skeleton.
+Require Import PCM.
+Require Import ModSem Behavior.
+Require Import Relation_Definitions.
+
+(*** TODO: export these in Coqlib or Universe ***)
+Require Import Relation_Operators.
+Require Import RelationPairs.
+From ITree Require Import
+     Events.MapDefault.
+From ExtLib Require Import
+     Core.RelDec
+     Structures.Maps
+     Data.Map.FMapAList.
+Require Import TODOYJ.
+
+Generalizable Variables E R A B C X Y.
+
+Set Implicit Arguments.
+
+Local Open Scope nat_scope.
+
+
+
+Notation "wf n '------------------------------------------------------------------' src0 tgt0 '------------------------------------------------------------------' src1 tgt1 '------------------------------------------------------------------' src2 tgt2"
+  :=
+    (gpaco3 (_sim_itree wf) _ _ _ n (([(_, src0)], src1), src2) (([(_, tgt0)], tgt1), tgt2))
+      (at level 60,
+       format "wf  n '//' '------------------------------------------------------------------' '//' src0 '//' tgt0 '//' '------------------------------------------------------------------' '//' src1 '//' tgt1 '//' '------------------------------------------------------------------' '//' src2 '//' '//' '//' tgt2 '//' ").
+
+
+
+Ltac prep := ired; try rewrite ! unfold_interp.
+
+Ltac force_l :=
+  prep;
+  match goal with
+  | [ |- (gpaco3 (_sim_itree _) _ _ _ _ (_, unwrapN ?ox >>= _) (_, _)) ] =>
+    let tvar := fresh "tmp" in
+    let thyp := fresh "TMP" in
+    remember (unwrapN ox) as tvar eqn:thyp; unfold unwrapN in thyp; subst tvar;
+    let name := fresh "_UNWRAPN" in
+    destruct (ox) eqn:name; [|exfalso]; cycle 1
+  | [ |- (gpaco3 (_sim_itree _) _ _ _ _ (_, guarantee ?P >>= _) (_, _)) ] =>
+    let tvar := fresh "tmp" in
+    let thyp := fresh "TMP" in
+    remember (guarantee P) as tvar eqn:thyp; unfold guarantee in thyp; subst tvar;
+    let name := fresh "_GUARANTEE" in
+    destruct (classic P) as [name|name]; [gstep; ired; eapply sim_itree_choose_src; [eauto|exists name]|contradict name]; cycle 1
+
+  | [ |- (gpaco3 (_sim_itree _) _ _ _ _ (_, ?i_src) (_, ?i_tgt)) ] =>
+    seal i_tgt; gstep; econs; eauto; unseal i_tgt
+  end
+.
+Ltac force_r :=
+  prep;
+  match goal with
+  | [ |- (gpaco3 (_sim_itree _) _ _ _ _ (_, _) (_, unwrapU ?ox >>= _)) ] =>
+    let tvar := fresh "tmp" in
+    let thyp := fresh "TMP" in
+    remember (unwrapU ox) as tvar eqn:thyp; unfold unwrapU in thyp; subst tvar;
+    let name := fresh "_UNWRAPU" in
+    destruct (ox) eqn:name; [|exfalso]; cycle 1
+  | [ |- (gpaco3 (_sim_itree _) _ _ _ _ (_, _) (_, assume ?P >>= _)) ] =>
+    let tvar := fresh "tmp" in
+    let thyp := fresh "TMP" in
+    remember (assume P) as tvar eqn:thyp; unfold assume in thyp; subst tvar;
+    let name := fresh "_ASSUME" in
+    destruct (classic P) as [name|name]; [gstep; ired; eapply sim_itree_take_tgt; [eauto|exists name]|contradict name]; cycle 1
+
+  | [ |- (gpaco3 (_sim_itree _) _ _ _ _ (_, ?i_src) (_, ?i_tgt)) ] =>
+    seal i_src; gstep; econs; eauto; unseal i_src
+  end
+.
+Ltac init :=
+  split; ss; ii; clarify; rename y into varg; eexists 100%nat; ss; des; clarify;
+  ginit; [eapply cpn3_wcompat; eauto with paco|]; unfold alist_add, alist_remove; ss;
+  unfold fun_to_tgt, cfun, HoareFun; ss.
+
+Ltac _step :=
+  match goal with
+  (*** blacklisting ***)
+  (* | [ |- (gpaco3 (_sim_itree wf) _ _ _ _ (_, trigger (Choose _) >>= _) (_, ?i_tgt)) ] => idtac *)
+  | [ |- (gpaco3 (_sim_itree _) _ _ _ _ (_, unwrapU ?ox >>= _) (_, _)) ] =>
+    let tvar := fresh "tmp" in
+    let thyp := fresh "TMP" in
+    remember (unwrapU ox) as tvar eqn:thyp; unfold unwrapU in thyp; subst tvar;
+    let name := fresh "_UNWRAPU" in
+    destruct (ox) eqn:name; [|unfold triggerUB; ired; _step; ss; fail]
+  | [ |- (gpaco3 (_sim_itree _) _ _ _ _ (_, assume ?P >>= _) (_, _)) ] =>
+    let tvar := fresh "tmp" in
+    let thyp := fresh "TMP" in
+    remember (assume P) as tvar eqn:thyp; unfold assume in thyp; subst tvar;
+    let name := fresh "_ASSUME" in
+    ired; gstep; eapply sim_itree_take_src; [apply Nat.lt_succ_diag_r|]; intro name
+
+  (*** blacklisting ***)
+  (* | [ |- (gpaco3 (_sim_itree wf) _ _ _ _ (_, _) (_, trigger (Take _) >>= _)) ] => idtac *)
+  | [ |- (gpaco3 (_sim_itree _) _ _ _ _ (_, _) (_, unwrapN ?ox >>= _)) ] =>
+    let tvar := fresh "tmp" in
+    let thyp := fresh "TMP" in
+    remember (unwrapN ox) as tvar eqn:thyp; unfold unwrapN in thyp; subst tvar;
+    let name := fresh "_UNWRAPN" in
+    destruct (ox) eqn:name; [|unfold triggerNB; ired; _step; ss; fail]
+  | [ |- (gpaco3 (_sim_itree _) _ _ _ _ (_, _) (_, guarantee ?P >>= _)) ] =>
+    let tvar := fresh "tmp" in
+    let thyp := fresh "TMP" in
+    remember (guarantee P) as tvar eqn:thyp; unfold guarantee in thyp; subst tvar;
+    let name := fresh "_GUARANTEE" in
+    ired; gstep; eapply sim_itree_choose_tgt; [apply Nat.lt_succ_diag_r|]; intro name
+
+
+
+  | _ => (*** default ***)
+    gstep; econs; try apply Nat.lt_succ_diag_r; i
+  end;
+  (* idtac *)
+  match goal with
+  | [ |- exists _, _ ] => fail 1
+  | _ => idtac
+  end
+.
+Ltac steps := repeat ((*** pre processing ***) prep; try _step; (*** post processing ***) unfold alist_add; simpl; des_ifs_safe).
+
+
+
+Section SIMMODSEM.
+
+  Context `{Σ: GRA.t}.
+  Context `{@GRA.inG Mem1.memRA Σ}.
+
+  Let W: Type := (alist mname (Σ * Any.t)) * (alist mname (Σ * Any.t)).
+  Eval compute in (@URA.car Mem1._memRA).
+
+  Let wf: W -> Prop :=
+    fun '(mrps_src0, mrps_tgt0) =>
+        (<<SRC: mrps_src0 = Maps.add "LinkedList" (ε, tt↑) Maps.empty>>) /\
+        (<<TGT: mrps_tgt0 = Maps.add "LinkedList" (ε, tt↑) Maps.empty>>)
+  .
+
+  Local Opaque points_to.
+
+  Hint Resolve sim_itree_mon: paco.
+
+  Opaque URA.unit.
+  Definition iApp (P: Σ -> Prop) (r: Σ): Prop := P r /\ URA.wf r.
+  (* Notation "'ᐸ ' P ' ᐳ'" := (iApp P _) (at level 60). (* (format "'ᐸ'  P  'ᐳ'") *) *)
+  Notation "'ᐸ' P 'ᐳ'" := (iApp P _) (at level 60). (* (format "'ᐸ'  P  'ᐳ'") *)
+  Goal forall a, (iApp (fun _ => True) a). Abort.
+
+  Lemma intro_iApp: forall P r, URA.wf r -> P r = iApp P r.
+    { i. unfold iApp. apply prop_ext. split; i; des; et. }
+  Qed.
+
+  Lemma wf_split: forall (a b: Σ), URA.wf (a ⋅ b) -> URA.wf a /\ URA.wf b.
+    { i. split; eapply URA.wf_mon; et. rewrite URA.add_comm; et. }
+  Qed.
+
+  Theorem correct: ModSemPair.sim LinkedList1.LinkedListSem LinkedList0.LinkedListSem.
+  Proof.
+    econstructor 1 with (wf:=wf) (le:=top2); et; swap 2 3.
+    { typeclasses eauto. }
+    { ss. }
+
+    econs; ss.
+    { init.
+      unfold checkWf, forge, discard, put. steps.
+      unfold popF. steps.
+      des. clarify.
+      r in _ASSUME0. des. r in _ASSUME0. des; subst. r in _ASSUME1. des; subst. r in _ASSUME0. des; subst.
+
+      Ltac on_first_hyp tac :=
+        match reverse goal with [ H : _ |- _ ] => first [ tac H | fail 1 ] end.
+
+      Ltac to_bar TAC :=
+        match goal with
+        | [H: bar_True |- _ ] => TAC H
+        | _ => idtac
+        end.
+      Ltac bar :=
+        to_bar ltac:(fun _ => fail 1);
+        let NAME := fresh "ㅡㅡㅡㅡㅡㅡㅡㅡㅡㅡㅡㅡㅡㅡㅡㅡㅡㅡㅡㅡㅡㅡㅡㅡㅡㅡㅡㅡㅡㅡㅡㅡㅡ" in
+        assert (NAME : bar_True) by ss
+      .
+
+      Ltac iSimplWf :=
+        repeat match goal with
+               | [H: URA.wf (?a ⋅ ?b) |- _ ] =>
+                 repeat (try rewrite URA.unit_id in H; try rewrite URA.unit_idl in H);
+                 apply wf_split in H; destruct H
+               end.
+
+      Ltac iRefresh :=
+        try bar;
+        iSimplWf;
+        repeat multimatch goal with
+               | [H: ?ip ?r |- _ ] =>
+                 match type of ip with
+                 | iProp =>
+                   match goal with
+                   | [G: URA.wf r |- _ ] =>
+                     rewrite intro_iApp in H; [|exact G]; clear G; move r at top; move H at bottom
+                   end
+                 | _ => idtac
+                 end
+               end.
+      iRefresh. iRefresh. Fail progress iRefresh. (*** test ***)
+      Ltac iPure H := rr in H; destruct H as [H _]; red in H; to_bar ltac:(fun BAR => move H after BAR). (* ; iRefresh. *)
+      iPure _ASSUME1. iPure _ASSUME2. subst.
+      rewrite Any.upcast_downcast in *. clarify. apply Any.upcast_inj in _ASSUME1. des. apply JMeq_eq in EQ0. clear EQ. clarify. seal bar_True. clear_tac.
+      steps.
+      des. clarify. rewrite Any.upcast_downcast in *. clarify. apply_all_once Any.upcast_inj. des. clarify. clear_tac.
+      steps.
+      unfold APC. unfold interp_hCallE_tgt. steps. force_l. exists 0. steps. force_l. esplits; eauto.
+      force_l. esplits; eauto. force_l.
+      set (blk := (Mem.nb mem_tgt)) in *.
+      rename x0 into sz. rename _ASSUME into WF.
+      set (mem_src_new := add_delta_to_black
+                            (URA.black (mem_src: URA.car (t:=Mem1._memRA)))
+                            (points_to (blk, 0%Z) (repeat (Vint 0) sz))).
+      eexists (GRA.padding (mem_src_new: URA.car (t:=Mem1.memRA)),
+               GRA.padding ((blk, 0%Z) |-> (repeat (Vint 0) sz))).
+      Local Opaque URA.add. steps.
+      assert(WFA: forall ofs, mem_src (Mem.nb mem_tgt) ofs = inr tt).
+      { i.
+        destruct (mem_src (Mem.nb mem_tgt) ofs) eqn:A; cycle 1.
+        { des_u; ss. }
+        destruct o.
+        - admit "ez - add tgt wf".
+        - admit "ez - inl None is boom in RA.excl".
+      }
+      rewrite URA.unit_idl in *. rewrite ! GRA.padding_add.
+      force_l.
+      { etrans.
+        { eapply URA.extends_updatable. eexists; et. }
+        eapply GRA.padding_updatable.
+        ss.
+        replace (URA.excl ((mem_src: URA.car (t:=Mem1._memRA)) ⋅ f) ε) with
+            (URA.black ((mem_src: URA.car (t:=Mem1._memRA)) ⋅ f)) by ss.
+        eapply URA.auth_alloc2.
+        eapply URA.wf_mon in WF.
+        eapply GRA.padding_wf in WF. des.
+        clear - WF WFA Heq NULLPTR SIM.
+        Local Transparent URA.add points_to.
+        ss. des. unfold URA.white in Heq. clarify.
+        ii. des_ifs; ss.
+        - bsimpl; des; des_sumbool; clarify.
+          exploit WFA; et. intro A. rewrite A in *; ss.
+        - specialize (WF0 k k0). bsimpl; des; des_sumbool; clarify; des_ifs.
+        - specialize (WF0 k k0). bsimpl; des; des_sumbool; clarify; des_ifs.
+          apply_all_once Z.leb_le. apply_all_once Z.ltb_lt.
+          intro A. apply nth_error_None in A. rewrite repeat_length in *.
+          apply inj_le in A. rewrite Z2Nat.id in A; cycle 1.
+          { lia. }
+          lia.
+        Local Opaque URA.add points_to.
+      }
+      Local Opaque URA.wf.
+      ss.
+      steps. force_l. esplits; eauto. force_l.
+      { esplits; eauto. }
+      steps.
+      force_l. esplits; eauto.
+      force_l.
+      { instantiate (1:= GRA.padding _). rewrite GRA.padding_add. rewrite URA.unit_id. f_equal. ss. }
+      clear _GUARANTEE0 _GUARANTEE1.
+      Local Opaque URA.add points_to.
+      Local Transparent points_to.
+      unfold points_to, URA.white in Heq. clarify. ss.
+      eapply URA.wf_mon in WF. eapply GRA.padding_wf in WF. des. ss. des. clear_tac. clear WF.
+      clear mem_src_new.
+      steps. esplits; ss; cycle 1.
+      - Local Transparent URA.add.
+        ss. des_ifs. bsimpl; des; des_sumbool; ss.
+        subst blk. clear - Heq1.
+        admit "ez: add tgt wf".
+        Local Opaque URA.add.
+      - ss. ii.
+        destruct (dec b blk).
+        + subst. unfold blk. unfold update. des_ifs_safe.
+          des_ifs.
+          * bsimpl; des; try rewrite Z.leb_le in *; try rewrite Z.ltb_lt in *.
+            Local Transparent URA.add.
+            s.
+            Local Opaque URA.add.
+            des_ifs; bsimpl; des; des_sumbool; ss; clarify; try rewrite Z.leb_le in *; try rewrite Z.ltb_lt in *;
+              try rewrite Z.leb_gt in *; try rewrite Z.ltb_ge in *; try lia; et.
+            { exploit WFA; et. intro A. rewrite A in *; ss. }
+            { exploit WFA; et. intro A. rewrite A in *; ss. }
+            { rewrite Z.sub_0_r.
+              destruct (nth_error (repeat (Vint 0) sz) (Z.to_nat ofs)) eqn:U.
+              - eapply nth_error_In in U. eapply repeat_spec in U. subst. econs; et.
+              - eapply nth_error_None in U. lia.
+            }
+            { rewrite repeat_length in *. lia. }
+          * Local Transparent URA.add.
+            s.
+            Local Opaque URA.add.
+            des_ifs; bsimpl; des; des_sumbool; ss; clarify; try rewrite Z.leb_le in *; try rewrite Z.ltb_lt in *;
+              try rewrite Z.leb_gt in *; try rewrite Z.ltb_ge in *; try lia; et;
+                try (by exploit WFA; et; intro A; rewrite A in *; ss).
+            { rewrite Z.sub_0_r. rewrite repeat_length in *. lia. }
+            { econs; eauto. }
+            { econs; eauto. }
+        + Local Transparent URA.add.
+          ss.
+          hexploit (SIM b ofs); et. intro A. inv A.
+          {
+            des_ifs; bsimpl; des; des_sumbool; clarify.
+            - unfold update. des_ifs. rewrite <- H1. econs.
+            - unfold update. des_ifs. rewrite <- H1. econs.
+            - unfold update. des_ifs. rewrite <- H1. econs.
+          }
+          {
+            des_ifs; bsimpl; des; des_sumbool; clarify.
+            - unfold update. des_ifs. rewrite <- H1. econs.
+            - unfold update. des_ifs. rewrite <- H1. econs.
+            - unfold update. des_ifs. rewrite <- H1. econs.
+          }
+    }
+    econs; ss.
+    { init.
+      Local Opaque URA.add URA.wf.
+      unfold checkWf, forge, discard, put. steps.
+      unfold freeF. steps. rewrite Any.upcast_downcast. steps.
+      (************** TODO: rename x3 into ASSUME *********************)
+      des. clarify. clear_tac. rewrite Any.upcast_downcast in *. clarify.
+      clear v x5. (************ TODO: WHY? *******************)
+      steps.
+      unfold interp_hCallE_tgt. steps. force_l. exists 0. steps.
+      apply_all_once Any.upcast_inj. des; clarify. clear_tac.
+      rewrite URA.unit_idl in *. rewrite GRA.padding_add in *. eapply GRA.padding_wf in x1. des.
+      rename x1 into WF.
+      rename n into b. rename z into ofs. rename v0 into v.
+
+      assert(A: mem_src b ofs = inl (Some v)).
+      { Local Transparent URA.wf.
+        ss. des_ifs. des. specialize (WF0 b ofs).
+        Local Transparent URA.add.
+        clear SIM.
+        Local Transparent URA.unit.
+        ss. clarify. rr in WF. des. clarify. ss.
+        des_ifs;
+          bsimpl; des; des_sumbool; ss;
+          repeat des_u;
+          clear_tac;
+          try rewrite Z.leb_le in *; try rewrite Z.leb_gt in *; try rewrite Z.ltb_lt in *; try rewrite Z.ltb_ge in *;
+          try rewrite Z.sub_diag in *;
+          try lia; ss.
+        Local Opaque URA.wf URA.add URA.unit.
+      }
+
+      set (mem_src' := fun _b _ofs => if dec _b b && dec _ofs ofs then inr () else mem_src _b _ofs).
+
+      assert(WF': URA.wf (mem_src': URA.car (t:=Mem1._memRA))).
+      { Local Transparent URA.add URA.wf.
+        ss. ii. des_ifs.
+        ss. clarify.
+        subst mem_src'. ss. des_ifs. des. specialize (WF0 k k0). bsimpl. des; des_sumbool; des_ifs.
+        Local Opaque URA.wf URA.add.
+      }
+      hexploit (SIM b ofs); et. intro B. rewrite A in *. inv B.
+      force_r.
+      { exfalso. unfold Mem.free in *. des_ifs. }
+      rename t into mem_tgt'.
+      assert(SIM': forall b ofs, sim_loc (Mem.cnts mem_tgt' b ofs) (mem_src' b ofs)).
+      { i.
+        unfold Mem.free in _UNWRAPU. des_ifs. ss.
+        subst mem_src'. ss.
+        destruct (classic (b = b0 /\ ofs = ofs0)); des; clarify.
+        - destruct H0; clarify. (**** TODO: FIX ****) unfold update. des_ifs. econs.
+        - des_ifs.
+          { Psimpl. bsimpl; des; des_sumbool; ss; clarify. destruct H0; ss. destruct H1; ss. (**** TODO: FIX ****)}
+          replace (update (Mem.cnts mem_tgt) b (update (Mem.cnts mem_tgt b) ofs None) b0 ofs0) with
+              (Mem.cnts mem_tgt b0 ofs0); cycle 1.
+          { unfold update. des_ifs. Psimpl. des_ifs; bsimpl; des; des_sumbool; ss; clarify. }
+          et.
+      }
+      force_l. esplits.
+      force_l. esplits. force_l.
+      eexists ((GRA.padding (URA.black (mem_src': URA.car (t:=Mem1._memRA)))), URA.unit: URA.car (t:=Σ)).
+      steps.
+      steps. force_l.
+      { rewrite URA.unit_id.
+        rewrite ! GRA.padding_add. apply GRA.padding_updatable.
+        apply URA.auth_dealloc.
+        clear - WF' WF.
+        r. i. rewrite URA.unit_idl.
+        ss. destruct H; clear H. (*** coq bug; des infloops ***) des. clarify.
+        esplits; et.
+        apply func_ext. intro _b. apply func_ext. intro _ofs.
+        destruct (classic (b = _b /\ ofs = _ofs)).
+        - destruct H; clear H. clarify.
+          subst mem_src'. ss. des_ifs; bsimpl; des; des_sumbool; clarify.
+          clear - H0.
+          Local Transparent URA.wf.
+          Local Transparent URA.add.
+          specialize (H0 _b _ofs). ss.
+          des_ifs; bsimpl; des; des_sumbool;
+            try rewrite Z.leb_le in *; try rewrite Z.leb_gt in *; try rewrite Z.ltb_lt in *; try rewrite Z.ltb_ge in *;
+              try rewrite Z.sub_diag in *;
+              try lia; ss.
+          des_u. ss.
+        - Psimpl.
+          subst mem_src'. s.
+          des_ifs; bsimpl; des; des_sumbool;
+            try rewrite Z.leb_le in *; try rewrite Z.leb_gt in *; try rewrite Z.ltb_lt in *; try rewrite Z.ltb_ge in *;
+              try rewrite Z.sub_diag in *;
+              try lia; ss.
+          Local Opaque URA.wf.
+          Local Opaque URA.add.
+      }
+      steps. force_l. esplits. force_l. { esplits; eauto. } steps. force_l. esplits. force_l.
+      { rewrite URA.unit_idl. ss. }
+      steps.
+      esplits; eauto.
+      admit "ez - add a condition in wf, so that points-to predicate containing Vnullptr is never published".
+    }
+    Local Opaque points_to URA.add URA.wf URA.unit.
+    econs.
+    { init.
+      unfold checkWf, forge, discard, put. steps.
+      unfold loadF. steps. rewrite Any.upcast_downcast. steps.
+      (************** TODO: rename x3 into ASSUME *********************)
+      des. clarify. clear_tac. rewrite Any.upcast_downcast in *. clarify.
+      apply_all_once Any.upcast_inj. des. clarify. clear_tac.
+      rewrite URA.unit_idl in *. rewrite GRA.padding_add in *. apply_all_once GRA.padding_wf. des.
+      ss.
+      unfold interp_hCallE_tgt. steps. force_l. exists 0. steps. force_l. esplit. force_l. esplit.
+      rename n into b. rename z into ofs.
+      force_l. eexists (GRA.padding (URA.black (mem_src: URA.car (t:=Mem1._memRA))),
+                        GRA.padding ((b, ofs) |-> [v])).
+      steps.
+      force_l. { refl. } steps. force_l. esplit. force_l. { esplits; eauto. } steps.
+      force_l. esplit. steps. force_l. { rewrite URA.unit_id. refl. } steps.
+      assert(T: mem_src b ofs = inl (Some v)).
+      { Local Transparent points_to URA.add URA.wf URA.unit.
+        clear - x1.
+        ss. des. do 2 spc x0. rr in x1. des. ss.
+        des_ifs; bsimpl; des; des_sumbool; ss;
+          try rewrite Z.leb_le in *; try rewrite Z.leb_gt in *; try rewrite Z.ltb_lt in *; try rewrite Z.ltb_ge in *;
+            try rewrite Z.sub_diag in *; try lia; ss.
+        Local Opaque points_to URA.add URA.wf URA.unit.
+      }
+      exploit SIM; et. intro U. rewrite T in U. inv U; ss. unfold Mem.load. force_r; ss. clarify. steps.
+      esplits; eauto.
+    }
+    econs.
+    { init.
+      unfold checkWf, forge, discard, put. steps.
+      unfold storeF. steps. rewrite Any.upcast_downcast. steps.
+      (************** TODO: rename x3 into ASSUME *********************)
+      des. clarify. clear_tac. rewrite Any.upcast_downcast in *. clarify.
+      apply_all_once Any.upcast_inj. des. clarify. clear_tac.
+      rewrite URA.unit_idl in *. rewrite GRA.padding_add in *. apply_all_once GRA.padding_wf. des.
+      ss.
+      unfold interp_hCallE_tgt. steps. force_l. exists 0. steps. force_l. esplit. force_l. esplit.
+      rename n into b. rename z into ofs.
+      set (mem_src' := fun _b _ofs => if dec _b b && dec _ofs ofs then inl (Some v) else mem_src _b _ofs).
+      force_l. eexists (GRA.padding (URA.black (mem_src': URA.car (t:=Mem1._memRA))),
+                        GRA.padding ((b, ofs) |-> [v])).
+      rename x1 into WF.
+      assert(WF0: URA.wf (mem_src': URA.car (t:=Mem1._memRA))).
+      { Local Transparent URA.wf.
+        clear - WF. apply URA.wf_mon in WF. ss. des.
+        ii. specialize (WF0 k k0). des_ifs_safe. unfold mem_src' in *. des_ifs.
+        Local Opaque URA.wf.
+      }
+      steps.
+      force_l.
+      { rewrite ! GRA.padding_add. eapply GRA.padding_updatable.
+        clear - WF WF0. clear WF.
+        Local Transparent URA.add GRA.to_URA points_to URA.wf URA.unit.
+        eapply URA.auth_update; et.
+        rr. ii. destruct H; clear H. (*** FIXME: des runs infloop ***)
+        des. subst. esplits; et.
+        subst mem_src'. do 2 (apply func_ext; i). specialize (H0 x x0). specialize (WF0 x x0). ss.
+        des_ifs; bsimpl; des; des_sumbool; ss; subst;
+          try rewrite Z.leb_le in *; try rewrite Z.leb_gt in *; try rewrite Z.ltb_lt in *; try rewrite Z.ltb_ge in *;
+            try rewrite Z.sub_diag in *; try lia; ss.
+        Local Opaque URA.add GRA.to_URA points_to URA.wf URA.unit.
+      }
+      steps. force_l. esplit. force_l. { esplits; eauto. } steps.
+      force_l. esplit. steps. force_l. { rewrite URA.unit_id. refl. } steps.
+      assert(v_old0 = v_old).
+      { admit "TODO----------FIXTHIS". }
+      subst.
+      assert(U: mem_src b ofs = inl (Some v_old)).
+      { Local Transparent URA.add GRA.to_URA points_to URA.wf URA.unit.
+        clear - WF. ss. des. specialize (WF0 b ofs). r in WF. des; clarify. ss.
+        des_ifs; bsimpl; des; des_sumbool; ss; subst;
+          try rewrite Z.leb_le in *; try rewrite Z.leb_gt in *; try rewrite Z.ltb_lt in *; try rewrite Z.ltb_ge in *;
+            try rewrite Z.sub_diag in *; try lia; ss.
+        Local Opaque URA.add GRA.to_URA points_to URA.wf URA.unit.
+      }
+      hexploit SIM; et. intro V. rewrite U in V. inv V; ss. unfold Mem.store. rewrite <- H1. steps.
+      esplits; eauto.
+      { esplits; ss; et. des_ifs.
+        - bsimpl; des; des_sumbool; ss; subst. unfold mem_src'. des_ifs; bsimpl; des; des_sumbool; ss. econs; et.
+        - unfold mem_src'. des_ifs. bsimpl; des; des_sumbool; subst; ss.
+      }
+      admit "ez - add a condition in wf, so that points-to predicate containing Vnullptr is never published".
+    }
+    econs; et.
+    { admit "MINKI!!!". }
+  Unshelve.
+    all: ss.
+    all: try (by repeat econs; et).
+  Qed.
+
+End SIMMODSEM.
+
+
